rules/rules_equality3.v
@@ -30,6 +30,8 @@
 *)
 
 
+Require Export sequents2.
+Require Export sequents_lib.
 Require Export rules_useful.
 Require Export per_props_equality.
 Require Export per_props_union.
@@ -205,4 +207,163 @@ Proof.
 
         { eapply cequivc_trans in d;[|eauto].
           right; spcast; auto. }
+Qed.
+
+
+
+Definition rule_equality_equality_concl {o} (H : @bhyps o) a1 a2 b1 b2 A B i :=
+  mk_baresequent
+    H
+    (mk_conclax (mk_equality
+                   (mk_equality a1 a2 A)
+                   (mk_equality b1 b2 B)
+                   (mk_uni i))).
+
+Definition rule_equality_equality_hyp1 {o} (H : @bhyps o) A B i e :=
+  mk_baresequent H (mk_concl (mk_equality A B (mk_uni i)) e).
+
+Definition rule_equality_equality_hyp2 {o} (H : @bhyps o) a b A e :=
+  mk_baresequent H (mk_concl (mk_equality a b A) e).
+
+(**
+
+<<
+   H |- (a1 = a2 in A) = (b1 = b2 in B) in U(i)
+
+     By equalityEquality
+
+     H |- A = B in U(i)
+     H |- a1 = b1 in A
+     H |- a2 = b2 in A
+>>
+ *)
+Definition rule_equality_equality {o}
+           (H  : @barehypotheses o)
+           (A B a1 a2 b1 b2 e1 e2 e3 : NTerm)
+           (i : nat) :=
+  mk_rule
+    (rule_equality_equality_concl H a1 a2 b1 b2 A B i)
+    [ rule_equality_equality_hyp1 H A B i e1,
+      rule_equality_equality_hyp2 H a1 b1 A e2,
+      rule_equality_equality_hyp2 H a2 b2 A e3
+    ]
+    [].
+
+Lemma rule_equality_equality_true3 {o} :
+  forall lib (H : @barehypotheses o)
+         (A B a1 a2 b1 b2 e1 e2 e3 : NTerm)
+         (i : nat),
+    rule_true3 lib (rule_equality_equality H A B a1 a2 b1 b2 e1 e2 e3 i).
+Proof.
+  unfold rule_equality_equality, rule_true3, wf_bseq, closed_type_baresequent, closed_extract_baresequent; simpl.
+  intros.
+  clear cargs.
+
+  (* We prove the well-formedness of things *)
+  destseq; allsimpl.
+  dLin_hyp.
+  destruct Hyp as [wf1 hyp1].
+  destruct Hyp0 as [wf2 hyp2].
+  destruct Hyp1 as [wf3 hyp3].
+  destseq; allsimpl; proof_irr; GC.
+
+  match goal with
+  | [ |- sequent_true2 _ ?s ] => assert (wf_csequent s) as wfc
+  end.
+  {
+    clear hyp1 hyp2 hyp3.
+    unfold wf_csequent, wf_sequent, wf_concl; simpl.
+    dands; auto.
+    - apply wf_axiom.
+    - unfold closed_extract; simpl; auto.
+  }
+  exists wfc.
+  destseq; simpl in *.
+
+  (* We prove some simple facts on our sequents *)
+  (* done with proving these simple facts *)
+
+  vr_seq_true.
+  lsubst_tac.
+  rw <- @member_equality_iff.
+
+  pose proof (teq_and_eq_if_equality
+                lib (mk_uni i) (mk_equality a1 a2 A) (mk_equality b1 b2 B)
+                s1 s2 H wT w1 w2 c1 c6 c2 c7 cT cT2
+                eqh sim) as eqp.
+  lsubst_tac.
+  repeat (autodimp eqp hyp);[apply tequality_mkc_uni|].
+
+  clear dependent s1.
+  clear dependent s2.
+
+  introv hf sim.
+  lsubst_tac.
+  apply equality_mkc_equality2_sp_in_uni; dands.
+
+  - vr_seq_true in hyp1.
+    pose proof (hyp1 s1 s2 hf sim) as h; clear hyp1; exrepnd.
+    lsubst_tac.
+    apply equality_in_mkc_equality in h1; repnd.
+    clear h1 h3.
+    apply equality_commutes in h0; auto.
+
+  - split; left.
+
+    + vr_seq_true in hyp2.
+      pose proof (hyp2 s1 s2 hf sim) as h; clear hyp2; exrepnd.
+      lsubst_tac.
+      rw @tequality_mkc_equality_sp in h0; repnd.
+      allrw @fold_equorsq.
+      apply equality_in_mkc_equality in h1; repnd.
+      eapply cequorsq_equality_trans2 in h4;[|eauto]; auto.
+
+    + vr_seq_true in hyp3.
+      pose proof (hyp3 s1 s2 hf sim) as h; clear hyp2; exrepnd.
+      lsubst_tac.
+      rw @tequality_mkc_equality_sp in h0; repnd.
+      allrw @fold_equorsq.
+      apply equality_in_mkc_equality in h1; repnd.
+      eapply cequorsq_equality_trans2 in h4;[|eauto]; auto.
+Qed.
+
+Lemma rule_equality_equality_true_ext_lib {o} :
+  forall lib (H : @barehypotheses o)
+         (A B a1 a2 b1 b2 e1 e2 e3 : NTerm)
+         (i : nat),
+    rule_true_ext_lib lib (rule_equality_equality H A B a1 a2 b1 b2 e1 e2 e3 i).
+Proof.
+  introv.
+  apply rule_true3_implies_rule_true_ext_lib.
+  introv.
+  apply rule_equality_equality_true3.
+Qed.
+
+Lemma rule_equality_equality_wf2 {o} :
+  forall (H : @barehypotheses o)
+         (A B a1 a2 b1 b2 e1 e2 e3 : NTerm)
+         (i : nat),
+    wf_rule2 (rule_equality_equality H A B a1 a2 b1 b2 e1 e2 e3 i).
+Proof.
+  introv wf m; allsimpl.
+  repndors; subst; tcsp;
+    allunfold @wf_bseq; allsimpl; repnd; dands; auto.
+
+  - allrw <- @wf_equality_iff; tcsp.
+
+  - unfold closed_type_baresequent in *; simpl in *.
+    unfold closed_type in *; simpl in *.
+    allrw @covered_equality; tcsp.
+
+  - allrw <- @wf_equality_iff; tcsp.
+
+  - unfold closed_type_baresequent in *; simpl in *.
+    unfold closed_type in *; simpl in *.
+    allrw @covered_equality; tcsp.
+
+  - allrw <- @wf_equality_iff; tcsp.
+
+  - unfold closed_type_baresequent in *; simpl in *.
+    unfold closed_type in *; simpl in *.
+    allrw @covered_equality; tcsp.
 Qed.
